ver2/checker.v
@@ -454,7 +454,7 @@ Qed.
 Definition optimizations_pipeline : opt_pipeline := 
   [ 
     OpEntry optimize_eval_sbinding optimize_eval_sbinding_snd;
-    OpEntry optimize_add_0_sbinding optimize_add_0_sbinding_snd;
+    OpEntry optimize_add_zero_sbinding optimize_add_zero_sbinding_snd;
     OpEntry optimize_not_not_sbinding optimize_not_not_sbinding_snd;
     OpEntry optimize_and_and1_sbinding optimize_and_and1_sbinding_snd;
     OpEntry optimize_and_and2_sbinding optimize_and_and2_sbinding_snd
