ver2/optimizations/sub_x_x.v
@@ -1,0 +1,200 @@
+Require Import bbv.Word.
+Require Import Nat. 
+Require Import Coq.NArith.NArith.
+
+Require Import Coq.Logic.FunctionalExtensionality.
+
+Require Import FORVES.constants.
+Import Constants.
+
+Require Import FORVES.symbolic_state.
+Import SymbolicState.
+
+Require Import FORVES.symbolic_state_eval.
+Import SymbolicStateEval.
+
+Require Import FORVES.symbolic_state_cmp.
+Import SymbolicStateCmp.
+
+Require Import FORVES.valid_symbolic_state.
+Import ValidSymbolicState.
+
+Require Import FORVES.execution_state.
+Import ExecutionState.
+
+Require Import FORVES.stack_operation_instructions.
+Import StackOpInstrs.
+
+Require Import FORVES.program.
+Import Program.
+
+Require Import FORVES.symbolic_state_cmp_impl.
+Import SymbolicStateCmpImpl.
+
+Require Import FORVES.symbolic_state_eval_facts.
+Import SymbolicStateEvalFacts.
+
+Require Import FORVES.valid_symbolic_state.
+Import ValidSymbolicState.
+
+Require Import FORVES.misc.
+Import Misc.
+
+Require Import FORVES.eval_common.
+Import EvalCommon.
+
+Require Import FORVES.concrete_interpreter.
+Import ConcreteInterpreter.
+
+Require Import FORVES.optimizations_def.
+Import Optimizations_Def.
+
+Require Import FORVES.optimizations_common.
+Import Optimizations_Common.
+
+Require Import List.
+Import ListNotations.
+
+
+Module Opt_sub_x_x.
+
+
+(* SUB(X,X) = 0 *)
+Definition optimize_sub_x_x_sbinding : opt_smap_value_type := 
+fun (val: smap_value) =>
+fun (fcmp: sstack_val_cmp_t) =>
+fun (sb: sbindings) =>
+fun (maxid: nat) =>
+fun (instk_height: nat) =>
+fun (ops: stack_op_instr_map) => 
+match val with
+| SymOp SUB [arg1; arg2] => 
+  if fcmp arg1 arg2 maxid sb maxid sb instk_height ops then
+    (SymBasicVal (Val WZero), true)
+  else 
+    (val, false)
+| _ => (val, false)
+end.
+
+
+
+Lemma optimize_sub_x_x_sbinding_smapv_valid:
+opt_smapv_valid_snd optimize_sub_x_x_sbinding.
+Proof.
+unfold opt_smapv_valid_snd.
+intros instk_height n fcmp sb val val' flag.
+intros Hvalid_smapv_val Hvalid_sb Hoptm_sbinding.
+unfold optimize_sub_x_x_sbinding in Hoptm_sbinding.
+destruct (val) as [basicv|pushtagv|label args|offset smem|key sstrg|
+  offset size smem] eqn: eq_val; try (
+    injection Hoptm_sbinding as eq_val' eq_flag;
+    rewrite <- eq_val';
+    assumption).
++ destruct label eqn: eq_label; try 
+      (injection Hoptm_sbinding as eq_val' eq_flag;
+      rewrite <- eq_val'; assumption).
+  (* SUB *)
+  destruct args as [|arg1 r1] eqn: eq_args; try 
+    (injection Hoptm_sbinding as eq_val' eq_flag;
+    rewrite <- eq_val'; assumption).
+  destruct r1 as [|arg2 r2] eqn: eq_r1; try 
+    (injection Hoptm_sbinding as eq_val' eq_flag;
+    rewrite <- eq_val'; assumption).
+  destruct r2 as [|arg3 r3] eqn: eq_r2; try 
+    (injection Hoptm_sbinding as eq_val' eq_flag;
+    rewrite <- eq_val'; assumption).
+  destruct (fcmp arg1 arg2 n sb n sb instk_height evm_stack_opm)
+    eqn: eq_fcmp_arg1_arg2.
+  * injection Hoptm_sbinding as eq_val' eq_flag.
+    rewrite <- eq_val'.
+    simpl. intuition.
+  * injection Hoptm_sbinding as eq_val' eq_flag.
+    rewrite <- eq_val'.
+    assumption.
+Qed.
+
+
+Lemma sub_x_x: forall (x: EVMWord), wminus x x = WZero.
+Proof. apply wminus_diag. Qed.
+
+
+Lemma optimize_sub_x_x_sbinding_snd:
+opt_sbinding_snd optimize_sub_x_x_sbinding.
+Proof.
+unfold opt_sbinding_snd.
+intros val val' fcmp sb maxidx instk_height idx flag Hsafe_sstack_val_cmp
+  Hvalid Hoptm_sbinding.
+split.
+- (* valid_sbindings *)
+  apply valid_bindings_snd_opt with (val:=val)(opt:=optimize_sub_x_x_sbinding)
+    (fcmp:=fcmp)(flag:=flag); try assumption.
+  apply optimize_sub_x_x_sbinding_smapv_valid. 
+    
+- (* evaluation is preserved *) 
+  intros stk mem strg ctx v Hlen Heval_orig.
+  assert (Hlen2 := Hlen).
+  rewrite -> Hlen in Hlen2.
+  rewrite <- Hlen in Hlen2 at 2.
+  unfold optimize_sub_x_x_sbinding in Hoptm_sbinding.
+  pose proof (Hvalid_maxidx instk_height maxidx idx val sb evm_stack_opm
+      Hvalid) as eq_maxidx_idx.
+  destruct val as [vv|vv|label args|offset smem|key sstrg|offset seze smem]
+    eqn: eq_val; try inject_rw Hoptm_sbinding eq_val'.
+  (* SymOp label args *)
+  destruct label; try inject_rw Hoptm_sbinding eq_val'.
+  destruct args as [|arg1 r1] eqn: eq_args; 
+    try inject_rw Hoptm_sbinding eq_val'.
+  destruct r1 as [|arg2 r2] eqn: eq_r1; 
+    try inject_rw Hoptm_sbinding eq_val'.
+  destruct r2 as [|arg3 r3] eqn: eq_r2; 
+    try inject_rw Hoptm_sbinding eq_val'.
+  destruct (fcmp arg1 arg2 idx sb idx sb instk_height) 
+    eqn: fcmp_arg1_arg2.
+  + (* arg1 ~ arg2 *)
+    injection Hoptm_sbinding as eq_val' _. 
+    rewrite <- eq_val'.
+    unfold eval_sstack_val.
+    rewrite <- eval_sstack_val'_freshvar.
+    rewrite -> eval_sstack_val'_const.
+    unfold eval_sstack_val in Heval_orig. simpl in Heval_orig.
+    rewrite -> PeanoNat.Nat.eqb_refl in Heval_orig.
+    simpl in Heval_orig.
+    destruct (eval_sstack_val' maxidx arg1 stk mem strg ctx idx sb evm_stack_opm)
+      as [varg1|] eqn: eval_arg1; try discriminate.
+    destruct (eval_sstack_val' maxidx arg2 stk mem strg ctx idx sb evm_stack_opm)
+      as [varg2|] eqn: eval_arg2; try discriminate.
+    (*unfold safe_sstack_val_cmp in Hsafe_sstack_val_cmp.*)
+
+    unfold valid_bindings in Hvalid.
+    destruct Hvalid as [eq_maxid [Hvalid_smap_value Hvalid_bindings_sb]].
+    unfold valid_smap_value in Hvalid_smap_value.
+    unfold valid_stack_op_instr in Hvalid_smap_value.
+    simpl in Hvalid_smap_value.
+    destruct (Hvalid_smap_value) as [_ [Hvalid_arg1 [Hvalid_arg2 _ ]]].
+    fold valid_bindings in Hvalid_bindings_sb.
+
+    pose proof (Hsafe_sstack_val_cmp arg1 arg2 idx sb idx sb 
+      instk_height evm_stack_opm Hvalid_arg1 Hvalid_arg2 Hvalid_bindings_sb
+      Hvalid_bindings_sb fcmp_arg1_arg2 stk mem strg ctx Hlen2)
+      as [vv [Heval_arg1 Heval_arg2]].
+    unfold eval_sstack_val in Heval_arg1.
+    unfold eval_sstack_val in Heval_arg2.
+    rewrite -> eq_maxidx_idx in Heval_arg1.
+    rewrite -> eq_maxidx_idx in Heval_arg2.
+    rewrite -> Heval_arg1 in eval_arg1.
+    rewrite -> Heval_arg2 in eval_arg2.
+    injection eval_arg1 as eq_varg1.
+    injection eval_arg2 as eq_varg2.
+    rewrite <- eq_varg1 in Heval_orig.
+    rewrite <- eq_varg2 in Heval_orig.
+    simpl in Heval_orig.
+    rewrite -> sub_x_x in Heval_orig.
+    assumption.
+  + (* arg1 ~/~ arg2 *)
+    injection Hoptm_sbinding as eq_val' _.
+    rewrite <- eq_val'.
+    assumption.
+Qed.
+
+
+End Opt_sub_x_x.
